new/golang/theory/array.v
@@ -1,0 +1,36 @@
+From Perennial.Helpers Require Import List ListLen Fractional NamedProps.
+From iris.algebra Require Import dfrac.
+From Perennial.iris_lib Require Import dfractional.
+From Perennial.goose_lang Require Import ipersist.
+From New.golang.defn Require Export slice.
+From New.golang.theory Require Import loop.
+From Perennial Require Import base.
+
+Section lemmas.
+Context `{ffi_sem: ffi_semantics} `{!ffi_interp ffi} `{!heapGS Σ} {core_sem : go.CoreSemantics}.
+
+Context `{!IntoVal V}.
+Context `{!TypedPointsto (Σ:=Σ) V}.
+Context `{!IntoValTyped V t}.
+
+Lemma own_array_nil ptr dq :
+  ⊢ ptr ↦{dq} (array.mk t 0 []).
+Proof.
+  rewrite typed_pointsto_unseal. simpl. iPureIntro. done.
+Qed.
+
+Lemma own_array_len ptr dq n vs :
+  ptr ↦{dq} (array.mk t n vs) -∗ ⌜ n = Z.of_nat $ length vs ⌝.
+Proof.
+  rewrite typed_pointsto_unseal. simpl. iIntros "[% _] !%". done.
+Qed.
+
+Lemma own_array_acc i dq n vs :
+  0 ≤ sint.Z i →
+  vs !! (sint.nat i) = Some v →
+  s ↦[t]*{dq} vs -∗
+  slice_index_ref t (sint.Z i) s ↦{dq} v ∗
+  (∀ v', slice_index_ref t (sint.Z i) s ↦{dq} v' -∗
+        s ↦[t]*{dq} (<[sint.nat i := v']> vs)).
+
+  ptr ↦{dq} (array.mk t n vs) -∗ ⌜ n = Z.of_nat $ length vs ⌝.
